Core/Metatheory/Rename.lean
@@ -1,0 +1,105 @@
+import LeanSubst
+import Core.Typing
+
+open LeanSubst
+
+theorem subst_lift [RenMap T] (σ : Subst T) :
+  x < n ->
+  rep Subst.lift σ n x = re x
+:= by
+  intro h; induction n generalizing x σ <;> simp [rep]
+  cases h
+  case _ n ih =>
+  cases x <;> simp [Subst.lift]
+  case _ i =>
+  have lem : i < n := by omega
+  replace ih := @ih i σ lem
+  rw [ih]
+
+theorem Kinding.closed_rep :
+  G;Δ ⊢ A : K ->
+  ∀ (σ : Subst Ty), A[rep Subst.lift σ Δ.length:_] = A
+:= by
+  intro j; induction j <;> intro σ <;> simp
+  case var Δ x K j =>
+    have lem : x < Δ.length := by sorry
+    rw [subst_lift σ lem]; simp
+  case arrow ih1 ih2 =>
+    rw [ih1 σ, ih2 σ]; simp
+  case all ih =>
+    replace ih := ih σ
+    simp at ih; exact ih
+  case app ih1 ih2 =>
+    rw [ih1 σ, ih2 σ]; simp
+  case eq ih1 ih2 =>
+    rw [ih1 σ, ih2 σ]; simp
+
+theorem Kinding.closed : G;[] ⊢ A : K -> ∀ σ, A[σ] = A := by
+  intro j; apply closed_rep j
+
+-- theorem GlobalWf.closed {G : List Global} :
+--   GlobalWf G g ->
+--   some T = g.type ->
+--   ∀ σ, T[σ] = T
+-- := by
+--   intro j h
+--   induction G
+--   sorry
+
+theorem Kinding.rename Δr (r : Ren) :
+  (∀ i, Δ[i]? = Δr[r i]?) ->
+  G;Δ ⊢ A : K ->
+  G;Δr ⊢ A[r] : K
+:= by
+  intro h j
+  induction j generalizing Δr r <;> simp
+  case var Δ x K j =>
+    simp [Ren.to]; apply Kinding.var
+    rw [h x] at j; exact j
+  case global j => apply Kinding.global j
+  case arrow ih1 ih2 => apply Kinding.arrow (ih1 _ _ h) (ih2 _ _ h)
+  case all K Δ P j ih =>
+    replace ih := ih (K::Δr) r.lift (by {
+      intro i; cases i <;> simp [Ren.lift]
+      case _ i => exact h i
+    })
+    rw [Ren.to_lift (S := Ty)] at ih; simp at ih
+    apply Kinding.all ih
+  case app ih1 ih2 => apply Kinding.app (ih1 _ _ h) (ih2 _ _ h)
+  case eq ih1 ih2 => apply Kinding.eq (ih1 _ _ h) (ih2 _ _ h)
+
+theorem Kinding.weaken : G;Δ ⊢ A : K -> G;(T::Δ) ⊢ A[+1] : K := by
+  intro j; apply rename (T::Δ) (· + 1) _ j
+  intro i; cases i <;> simp
+
+theorem Typing.rename_type Δr (r : Ren) :
+  (∀ i, Δ[i]? = Δr[r i]?) ->
+  G;Δ,Γ ⊢ t : A ->
+  G;Δr,Γ.map (·[r]) ⊢ t[r:Ty] : A[r]
+:= by
+  intro h j; induction j generalizing Δr r <;> simp
+  case var j1 j2 =>
+    apply Typing.var
+    simp; apply Exists.intro _
+    apply And.intro j1 rfl
+    apply Kinding.rename _ r h j2
+  case global j1 j2 =>
+    sorry
+  case mtch => sorry
+  case guard => sorry
+  case lam => sorry
+  case app => sorry
+  case lamt => sorry
+  case appt => sorry
+  case cast => sorry
+  case refl => sorry
+  case sym => sorry
+  case seq => sorry
+  case appc => sorry
+  case arrowc => sorry
+  case fst => sorry
+  case snd => sorry
+  case allc => sorry
+  case apptc => sorry
+  case zero => sorry
+  case choice => sorry
