Core/Term/Spine.lean
@@ -1,4 +1,5 @@
 import LeanSubst
+import Core.Util
 import Core.Term.Definition
 import Core.Term.Beq
 
@@ -8,6 +9,7 @@ inductive SpineElem : Type where
 | type (x : Ty)
 | term (x : Term)
 | oterm (x : Term)
+deriving Repr
 
 def SpineElem.beq : SpineElem -> SpineElem -> Bool
 | type A, type B => A == B
@@ -36,3 +38,80 @@ def Term.apply (t : Term) : List SpineElem -> Term
 | .cons (.type A) tl => (t •[A]).apply tl
 | .cons (.term a) tl => (t • a).apply tl
 | .cons (.oterm a) tl => (t ∘[a]).apply tl
+
+macro "spine_app_eq_solve" x:term : tactic => `(tactic| {
+  apply Iff.intro <;> intro h
+  case _ =>
+    simp [Term.spine] at h
+    replace h := Eq.symm h
+    rw [Option.bind_eq_some_iff] at h
+    rcases h with ⟨q, e1, e2⟩
+    rcases q with ⟨y, sp'⟩; simp at e2
+    rcases e2 with ⟨e2, e3⟩; subst e2 e3
+    rw [e1]; exists sp'
+  case _ =>
+    rcases h with ⟨sp', e1, e2⟩; subst e1
+    simp [Term.spine]; apply Eq.symm
+    rw [Option.bind_eq_some_iff]; apply Exists.intro ($x, sp')
+    apply And.intro (Eq.symm e2); simp
+})
+
+@[simp]
+theorem Spine.app_closed_eq {f a : Term} :
+  some (x, sp) = (f • a).spine
+  <-> ∃ sp', sp = sp' ++ [.term a] ∧ some (x, sp') = f.spine
+:= by spine_app_eq_solve x
+
+@[simp]
+theorem Spine.app_open_eq {f a : Term} :
+  some (x, sp) = (f ∘[a]).spine
+  <-> ∃ sp', sp = sp' ++ [.oterm a] ∧ some (x, sp') = f.spine
+:= by spine_app_eq_solve x
+
+@[simp]
+theorem Spine.appt_eq {f : Term} :
+  some (x, sp) = (f •[a]).spine
+  <-> ∃ sp', sp = sp' ++ [.type a] ∧ some (x, sp') = f.spine
+:= by spine_app_eq_solve x
+
+macro "spine_apply_solve" sp:Lean.Parser.Tactic.elimTarget "," t:term : tactic => `(tactic| {
+  induction $sp generalizing $t <;> simp [Term.apply]
+  case cons hd tl ih _ =>
+  cases hd <;> simp [Term.apply]
+  all_goals rw [ih]
+})
+
+theorem Spine.apply_term {t : Term} : t.apply sp • a = t.apply (sp ++ [.term a]) := by
+  spine_apply_solve sp, t
+
+theorem Spine.apply_oterm {t : Term} : t.apply sp ∘[a] = t.apply (sp ++ [.oterm a]) := by
+  spine_apply_solve sp, t
+
+theorem Spine.apply_type {t : Term} : t.apply sp •[a] = t.apply (sp ++ [.type a]) := by
+  spine_apply_solve sp, t
+
+macro "spine_apply_eq_case_solve"
+  h:term ","
+  ih:term ","
+  ap:Lean.Parser.Tactic.rwRule : tactic =>
+`(tactic| {
+  replace h := Eq.symm $h
+  rw [Option.bind_eq_some_iff] at h
+  rcases h with ⟨q, e1, e2⟩
+  rcases q with ⟨y, sp'⟩; simp at e2
+  rcases e2 with ⟨e2, e3⟩; subst e2 e3
+  replace ih := $ih (Eq.symm e1)
+  rw [ih, $ap]
+})
+
+theorem Spine.apply_eq  :
+  some (x, sp) = t.spine -> t = (g#x).apply sp
+:= by
+  intro h
+  fun_induction Term.spine generalizing x sp <;> simp at *
+  case _ y =>
+    rcases h with ⟨e1, e2⟩; subst e1 e2
+    simp [Term.apply]
+  case _ ih => spine_apply_eq_case_solve h, ih, apply_term
+  case _ ih => spine_apply_eq_case_solve h, ih, apply_oterm
+  case _ ih => spine_apply_eq_case_solve h, ih, apply_type
