Core/Term/Variant.lean
@@ -1,0 +1,8 @@
+import LeanSubst
+import Core.Term.Definition
+
+open LeanSubst
+
+def Term.not_choice : Term -> Bool
+| ctor2 .choice _ _ => false
+| _ => true
